theories/linear/code.v
@@ -1,0 +1,600 @@
+From iris.algebra Require Import excl auth list.
+From iris.bi.lib Require Import fractional.
+From iris.base_logic.lib Require Import invariants ghost_var mono_nat.
+From chase_lev Require Import atomic.
+From iris.proofmode Require Import proofmode.
+From iris.heap_lang Require Import proofmode notation.
+From iris.prelude Require Import options.
+From chase_lev Require Import mono_list.
+From chase_lev.linear Require Import helpers.
+
+Definition CAP_CONST : nat := 10.
+
+(*
+  We use a finite length list without resizing;
+  The push function diverges if bot gets out of bound.
+  +--+--+--+--+--+--+--+--
+  |99|10|20|30|40|  |  |   ..
+  +--+--+--+--+--+--+--+--
+      ^           ^
+      |           |
+      top         bot
+*)
+
+Section code.
+  Definition new_deque : val :=
+    λ: <>,
+      let: "array" := AllocN #CAP_CONST #0 in
+      ("array", ref #1, ref #1). (* array, top, bottom *)
+  
+  Definition arr : val := λ: "deque", Fst (Fst "deque").
+  Definition top : val := λ: "deque", Snd (Fst "deque").
+  Definition bot : val := λ: "deque", Snd "deque".
+  Definition loop : val := (rec: "loop" "x" := "loop" "x").
+  
+  Definition push : val :=
+    λ: "deque" "v",
+      let: "array" := arr "deque" in
+      let: "b" := !(bot "deque") in
+      if: #CAP_CONST ≤ "b" then loop #() else
+      "array" +ₗ "b" <- "v" ;;
+      bot "deque" <- "b" + #1.
+  
+  (* TODO: change to NONE/SOME *)
+  Definition pop : val :=
+    λ: "deque",
+      let: "array" := arr "deque" in
+      let: "b" := !(bot "deque") - #1 in
+      bot "deque" <- "b" ;;
+      let: "t" := !(top "deque") in
+      if: "b" < "t" then (* empty pop *)
+        bot "deque" <- "t" ;; (#false, #())
+      else let: "v" := !("array" +ₗ "b") in
+      if: "t" < "b" then (#true, "v") (* normal case *)
+      else let: "ok" := CAS (top "deque") "t" ("t" + #1) in
+      bot "deque" <- "t" + #1 ;;
+      if: "ok" then (#true, "v") (* popped *)
+      else (#false, #()). (* stolen *)
+
+  (* NOTE: b ≤ t doesn't necessarily mean the deque was empty!
+    It can also be the case that there was one element and
+    the owner thread prematurely decremented b trying to pop. *)
+  (* TODO: change to NONE/SOME *)
+  Definition steal : val :=
+    λ: "deque",
+      let: "array" := arr "deque" in
+      let: "t" := !(top "deque") in
+      let: "b" := !(bot "deque") in
+      if: "b" ≤ "t" then (#false, #()) (* too small to steal *)
+      else let: "v" := !("array" +ₗ "t") in
+      if: CAS (top "deque") "t" ("t" + #1)
+      then (#true, "v") (* success *)
+      else (#false, #()). (* fail *)
+End code.
+
+Class dequeG Σ := DequeG {
+    deque_tokG :> ghost_varG Σ (list val);
+    deque_popG :> ghost_varG Σ bool;
+    mono_listG :> mono_listG val Σ;
+    mono_natG :> mono_natG Σ
+  }.
+Definition dequeΣ : gFunctors :=
+  #[ghost_varΣ (list val);
+    ghost_varΣ bool;
+    mono_listΣ val;
+    mono_natΣ
+  ].
+Global Instance subG_dequeΣ {Σ} : subG dequeΣ Σ → dequeG Σ.
+Proof. solve_inG. Qed.
+
+Section RA.
+  Context `{!heapGS Σ, !dequeG Σ} (N : namespace).
+  Notation iProp := (iProp Σ).
+
+  Definition definite t b := t + (if decide (t < b) then 1 else 0).
+
+  Definition mono_deque_auth_own (γm : gname) (l : list val) (t b : nat) : iProp :=
+    ∃ (γl γtb : gname),
+    ⌜γm = encode (γl, γtb)⌝ ∗
+    ⌜1 ≤ t ≤ b ≤ CAP_CONST ∧ length l = CAP_CONST⌝ ∗
+    mono_list_auth_own γl 1 (take (definite t b) l) ∗
+    mono_nat_auth_own γtb 1 t.
+
+  Definition mono_deque_lb_own (γm : gname) (l : list val) (t b : nat) : iProp :=
+    ∃ (γl γtb : gname),
+    ⌜γm = encode (γl, γtb)⌝ ∗
+    ⌜1 ≤ t ≤ b ≤ CAP_CONST ∧ length l = CAP_CONST⌝ ∗
+    mono_list_lb_own γl (take (definite t b) l) ∗
+    mono_nat_lb_own γtb t.
+
+  Lemma mono_deque_own_alloc l :
+    ⌜length l = CAP_CONST⌝ ==∗ ∃ γ, mono_deque_auth_own γ l 1 1.
+  Proof.
+    iIntros (H).
+    iMod (mono_list_own_alloc (take 1 l)) as (γl) "[L _]".
+    iMod (mono_nat_own_alloc 1) as (γtb) "[N _]".
+    iExists (encode (γl, γtb)). iModIntro.
+    iExists _,_. iSplit; iFrame; auto.
+    iPureIntro. unfold CAP_CONST. split; auto. lia.
+  Qed.
+
+  Lemma mono_deque_get_lb γm l t b :
+    mono_deque_auth_own γm l t b -∗
+    mono_deque_lb_own γm l t b.
+  Proof.
+    iIntros "(%γl & %γtb & %ENC & %BOUND & L & N)".
+    iDestruct (mono_list_lb_own_get with "L") as "#Llb".
+    iDestruct (mono_nat_lb_own_get with "N") as "#Nlb".
+    iExists _,_. repeat iSplit; auto. all: iPureIntro; lia.
+  Qed.
+
+  Lemma mono_deque_auth_lb_length γm l1 t1 b1 l2 t2 b2 :
+    mono_deque_auth_own γm l1 t1 b1 -∗ mono_deque_lb_own γm l2 t2 b2 -∗
+    ⌜definite t2 b2 ≤ definite t1 b1⌝.
+  Proof.
+    iIntros "(%γl & %γtb & %ENC & %BOUND & L & N)".
+    iIntros "(%γl' & %γtb' & %ENC' & %BOUND' & L' & N')".
+      rewrite ENC in ENC'. apply (inj encode) in ENC'.
+      injection ENC' as [= <- <-].
+    iDestruct (mono_list_auth_lb_valid with "L L'") as "[_ %Pref]".
+    apply prefix_length in Pref. do 2 rewrite take_length in Pref.
+    unfold definite in *. do 2 case_decide; iPureIntro; lia.
+  Qed.
+
+  Lemma mono_deque_definite_length γm l t b :
+    mono_deque_lb_own γm l t b -∗ ⌜definite t b ≤ b ≤ length l⌝.
+  Proof.
+    iIntros  "(%γl & %γtb & %ENC & [%BOUND1 %BOUND2] & L & N)".
+    unfold definite. case_decide; iPureIntro; try lia.
+  Qed.
+
+  Lemma mono_deque_auth_lb_top γm l1 t1 b1 l2 t2 b2 :
+    mono_deque_auth_own γm l1 t1 b1 -∗ mono_deque_lb_own γm l2 t2 b2 -∗
+    ⌜t2 ≤ t1 ∧ (t1 = t2 → t2 < b2 → t1 < b1)⌝.
+  Proof.
+    iIntros "D1 D2".
+    iDestruct (mono_deque_auth_lb_length with "D1 D2") as "%D".
+    iDestruct "D1" as "(%γl & %γtb & %ENC & %BOUND & L & N)".
+    iDestruct "D2" as "(%γl' & %γtb' & %ENC' & %BOUND' & L' & N')".
+      rewrite ENC in ENC'. apply (inj encode) in ENC'.
+      injection ENC' as [= <- <-].
+    iDestruct (mono_nat_lb_own_valid with "N N'") as "[_ %Le]".
+    unfold definite in *. do 2 case_decide; iPureIntro; lia.
+  Qed.
+
+  Lemma mono_deque_lb_lookup γm i l1 t1 b1 l2 t2 b2 :
+    i < (definite t1 b1) → i < (definite t2 b2) →
+    mono_deque_lb_own γm l1 t1 b1 -∗ mono_deque_lb_own γm l2 t2 b2 -∗
+    ⌜l1 !! i = l2 !! i⌝.
+  Proof.
+    iIntros (Hi Hv) "D1 D2".
+      iDestruct (mono_deque_definite_length with "D1") as "%L1".
+      iDestruct (mono_deque_definite_length with "D2") as "%L2".
+    iDestruct "D1" as "(%γl & %γtb & %ENC & %BOUND & L & N)".
+    iDestruct "D2" as "(%γl' & %γtb' & %ENC' & %BOUND' & L' & N')".
+      rewrite ENC in ENC'. apply (inj encode) in ENC'.
+      injection ENC' as [= <- <-].
+    rewrite <- (lookup_take l1 (definite t1 b1)) by lia.
+      assert (is_Some (take (definite t1 b1) l1 !! i)) as [v1 Hv1].
+      { rewrite lookup_lt_is_Some take_length. lia. }
+    rewrite <- (lookup_take l2 (definite t2 b2)) by lia.
+      assert (is_Some (take (definite t2 b2) l2 !! i)) as [v2 Hv2].
+      { rewrite lookup_lt_is_Some take_length. lia. }
+    iDestruct (mono_list_lb_valid with "L L'") as "%Pref".
+    destruct Pref.
+    - rewrite Hv1. erewrite prefix_lookup; eauto.
+    - rewrite Hv2. erewrite prefix_lookup; eauto.
+  Qed.
+
+  Lemma mono_deque_auth_insert γm l t b i v :
+    (definite t b) ≤ i →
+    mono_deque_auth_own γm l t b -∗
+    mono_deque_auth_own γm (<[i:=v]> l) t b.
+  Proof.
+    iIntros (H) "(%γl & %γtb & %ENC & %BOUND & L & N)".
+    iExists _,_. repeat iSplit; auto. all: try iPureIntro; try lia.
+    1: rewrite insert_length; lia.
+    rewrite take_insert; auto. iFrame.
+  Qed.
+
+  Lemma mono_deque_update_top γm t2 l t1 b :
+    t1 ≤ t2 ≤ b →
+    mono_deque_auth_own γm l t1 b ==∗ mono_deque_auth_own γm l t2 b.
+  Proof.
+    iIntros (H) "(%γl & %γtb & %ENC & %BOUND & L & N)".
+    iMod (mono_list_auth_own_update (take (definite t2 b) l) with "L") as "[L _]".
+      { apply prefix_take. unfold definite. do 2 case_decide; lia. }
+    iMod (mono_nat_own_update t2 with "N") as "[N _]". 1: lia.
+    iModIntro.
+    iExists _,_. repeat iSplit; auto; iFrame.
+    all: iPureIntro; try lia.
+  Qed.
+
+  Lemma mono_deque_update_bot γm b2 l t b1 :
+    b1 ≤ b2 ≤ CAP_CONST ∨ t < b2 ≤ CAP_CONST →
+    mono_deque_auth_own γm l t b1 ==∗ mono_deque_auth_own γm l t b2.
+  Proof.
+    iIntros (H) "(%γl & %γtb & %ENC & %BOUND & L & N)".
+    iMod (mono_list_auth_own_update (take (definite t b2) l) with "L") as "[L _]".
+      { apply prefix_take. unfold definite. do 2 case_decide; lia. }
+    iModIntro.
+    iExists _,_. repeat iSplit; auto; iFrame.
+    all: iPureIntro; try lia.
+  Qed.
+End RA.
+
+Section proof.
+  Context `{!heapGS Σ, !dequeG Σ} (N : namespace).
+  Notation iProp := (iProp Σ).
+
+  (* TODO: change l to ↦∗{#1} & make another ghost_var in deque_content?
+     (see msqueue) *)
+  Definition deque_inv (γq γpop γm : gname) (arr top bot : loc) : iProp :=
+    ∃ (t b : nat) (l : list val) (Popping : bool),
+      let bp := if Popping then b-1 else b in
+      ⌜1 ≤ t ≤ b ≤ CAP_CONST ∧ length l = CAP_CONST⌝ ∗
+      top ↦ #t ∗ bot ↦{#1/2} #bp ∗ arr ↦∗{#1/2} l ∗
+      ghost_var γq (1/2) (slice l t b) ∗
+      ghost_var γpop (1/2) Popping ∗
+      mono_deque_auth_own γm l t b.
+
+  Definition is_deque (γq γpop γm : gname) (q : val) : iProp :=
+    ∃ (arr top bot : loc),
+      ⌜q = (#arr, #top, #bot)%V⌝ ∗
+      inv N (deque_inv γq γpop γm arr top bot).
+  Global Instance is_deque_persistent γq γpop γm q :
+    Persistent (is_deque γq γpop γm q) := _.
+
+  Definition deque_content (γq : gname) (frag : list val) : iProp :=
+    ghost_var γq (1/2) frag.
+
+  Definition own_deque (γq γpop : gname) (q : val) : iProp :=
+    ∃ (arr top bot : loc) (b : nat) (l : list val),
+      ⌜q = (#arr, #top, #bot)%V⌝ ∗
+      ⌜length l = CAP_CONST⌝ ∗
+      ghost_var γpop (1/2) false ∗
+      bot ↦{#1/2} #b ∗ arr ↦∗{#1/2} l.
+  
+  Lemma loop_spec v :
+    {{{ True }}} loop #v {{{ RET #(); False }}}.
+  Proof.
+    iIntros (Φ) "_ HΦ". wp_rec. iLöb as "IH". wp_rec.
+    by iApply "IH".
+  Qed.
+
+  Ltac fr :=
+    repeat iExists _;
+    try iFrame "arr↦"; try iFrame "arr↦1"; try iFrame "arr↦2"; 
+    iFrame; eauto.
+  Ltac autoall :=
+    eauto;
+    unfold CAP_CONST in *; unfold helpers.CAP_CONST in *;
+    unfold definite;
+    try by (
+      repeat iNext; repeat iIntros; repeat intros;
+      try case_decide; try iPureIntro;
+      try rewrite lookup_lt_is_Some;
+      try rewrite Qp.half_half;
+      try lia; done
+    ).
+
+  Lemma new_deque_spec :
+    {{{ True }}}
+      new_deque #()
+    {{{ γq γpop γm q, RET q;
+      is_deque γq γpop γm q ∗ deque_content γq [] ∗
+      own_deque γq γpop q
+    }}}.
+  Proof with autoall.
+    iIntros (Φ) "_ HΦ".
+    wp_lam. wp_alloc arr as "[arr↦1 arr↦2]"...
+    wp_pures. wp_alloc b as "[b↦1 b↦2]". wp_alloc t as "t↦".
+    iMod (ghost_var_alloc []) as (γq) "[γq1 γq2]".
+    iMod (ghost_var_alloc false) as (γpop) "[γpop1 γpop2]".
+    iMod (mono_deque_own_alloc (replicate (Z.to_nat CAP_CONST) #0)
+      with "[]") as (γm) "γm"...
+    iMod (inv_alloc N _ (deque_inv γq γpop γm arr t b)
+      with "[t↦ b↦1 arr↦1 γq1 γpop1 γm]") as "Inv".
+    { fr. rewrite replicate_length... }
+    wp_pures. iModIntro. iApply "HΦ". iSplit; fr.
+    iExists _,_,_,1,_. fr.
+  Qed.
+
+  Lemma push_spec γq γpop γm q (v : val) :
+    is_deque γq γpop γm q -∗
+    own_deque γq γpop q -∗
+    <<< ∀∀ l : list val, deque_content γq l >>>
+      push q v @ ↑N
+    <<< deque_content γq (l ++ [v]),
+      RET #(), own_deque γq γpop q >>>.
+  Proof with autoall.
+    iIntros "#Is Own" (Φ) "AU".
+      iDestruct "Own" as (arr top bot b l) "(-> & %HL & γ👑 & b👑 & arr👑)".
+      iDestruct "Is" as (arr' top' bot') "[%Is Inv]".
+      injection Is as [= <- <- <-].
+    wp_lam. unfold code.arr, code.bot. wp_pures.
+
+    (* load bot *)
+    wp_load. wp_pures.
+    case_bool_decide as HbC. { wp_pures. iApply loop_spec... }
+    wp_pures.
+
+    (* store value *)
+    wp_bind (_ <- _)%E.
+    iInv "Inv" as (t1 b1 l1 Pop1)
+      ">(%BOUND1 & t↦ & b↦ & arr↦ & γq & γpop & MD)".
+      iDestruct (ghost_var_agree with "γ👑 γpop") as "%". subst.
+      iDestruct (mapsto_agree with "b↦ b👑") as "%".
+        injection H as [=]. apply Nat2Z.inj in H.
+      iDestruct (array_agree with "arr↦ arr👑") as "%"... subst.
+    iDestruct (mono_deque_auth_insert _ _ _ _ b v with "MD") as "MD"...
+    iCombine "arr↦ arr👑" as "arr↦".
+      iApply (wp_store_offset with "arr↦")...
+      iNext. iIntros "[arr↦ arr👑]". iModIntro.
+    iSplitL "t↦ b↦ arr↦ γq γpop MD".
+    { fr. rewrite slice_insert_right... rewrite insert_length... }
+    wp_pures.
+    replace (Z.of_nat b + 1)%Z with (Z.of_nat (S b))...
+
+    (* store bot *)
+    iInv "Inv" as (t2 b2 l2 Pop2)
+      ">(%BOUND2 & t↦ & b↦ & arr↦ & γq & γpop & MD)".
+      iDestruct (ghost_var_agree with "γ👑 γpop") as "%". subst.
+      iDestruct (mapsto_agree with "b↦ b👑") as "%".
+        injection H as [=]. apply Nat2Z.inj in H.
+      iDestruct (array_agree with "arr↦ arr👑") as "%"; subst.
+        1: rewrite insert_length...
+    iMod "AU" as (l') "[Cont [_ Commit]]".
+      unfold deque_content.
+      iDestruct (ghost_var_agree with "γq Cont") as "%". subst.
+      rewrite <- slice_extend_right... 2: rewrite list_lookup_insert...
+    iCombine "b↦ b👑" as "b↦". wp_store.
+      iDestruct "b↦" as "[b↦ b👑]".
+    iMod (ghost_var_update_2 (slice (<[b:=v]> l) t2 (S b))
+      with "γq Cont") as "[γq Cont]"...
+    iMod (mono_deque_update_bot _ (S b) with "MD") as "MD"...
+    iMod ("Commit" with "Cont") as "Φ".
+    iModIntro. iModIntro.
+
+    iSplitL "t↦ b↦ arr↦ γq γpop MD". 1: fr...
+    iApply "Φ". fr. fr... iSplit...
+  Qed.
+
+  Lemma pop_spec γq γpop γm q :
+    is_deque γq γpop γm q -∗
+    own_deque γq γpop q -∗
+    <<< ∀∀ l : list val, deque_content γq l >>>
+      pop q @ ↑N
+    <<< ∃∃ (l' : list val) (b : bool) (v : val),
+        deque_content γq l' ∗
+        ⌜l = if b then l'++[v] else l'⌝ ,
+      RET (#b, v), own_deque γq γpop q >>>.
+  Proof with autoall.
+    iIntros "#Is Own" (Φ) "AU".
+      iDestruct "Own" as (arr top bot b l) "(-> & %HL & γ👑 & b👑 & arr👑)".
+      iDestruct "Is" as (arr' top' bot') "[%Is Inv]".
+      injection Is as [= <- <- <-].
+    wp_lam. unfold code.arr, code.top, code.bot. wp_pures.
+
+    (* load bot *)
+    wp_load. wp_pures.
+
+    (* decrement b early *)
+    wp_bind (_ <- _)%E.
+    iInv "Inv" as (t1 b1 l1 Pop2)
+      ">(%BOUND1 & t↦ & b↦ & arr↦ & γq & γpop & MD)".
+      iDestruct (ghost_var_agree with "γ👑 γpop") as "%". subst.
+      iDestruct (mapsto_agree with "b↦ b👑") as "%".
+        injection H as [=]. apply Nat2Z.inj in H.
+      iDestruct (array_agree with "arr↦ arr👑") as "%"... subst.
+    iCombine "b↦ b👑" as "b↦". wp_store.
+      replace (Z.of_nat b-1)%Z with (Z.of_nat (b-1))...
+      iDestruct "b↦" as "[b↦ b👑]".
+      iMod (ghost_var_update_2 true with "γ👑 γpop") as "[γ👑 γpop]"...
+    iModIntro. iSplitL "t↦ b↦ arr↦ γpop γq MD". 1: fr.
+    wp_pures.
+
+    (* load top *)
+    wp_bind (! _)%E.
+    iInv "Inv" as (t2 b2 l2 Pop1)
+      ">(%BOUND2 & t↦ & b↦ & arr↦ & γq & γpop & MD)".
+      iDestruct (ghost_var_agree with "γ👑 γpop") as "%". subst.
+      iDestruct (mapsto_agree with "b↦ b👑") as "%".
+        injection H as [=]. assert (b = b2)... subst. clear H.
+      iDestruct (array_agree with "arr↦ arr👑") as "%"... subst.
+    (* if t < b-1, this load is the commit point *)
+    destruct (decide (t2 < b2-1)).
+    { iMod "AU" as (l') "[Cont [_ Commit]]".
+        unfold deque_content.
+        iDestruct (ghost_var_agree with "Cont γq") as "%". subst.
+      assert (is_Some (l !! (b2-1))) as [v Hv]...
+        erewrite slice_shrink_right...
+      wp_load.
+      iMod (ghost_var_update_2 (slice l t2 (b2-1)) with "Cont γq") as "[Cont γq]"...
+        iMod (ghost_var_update_2 false with "γ👑 γpop") as "[γ👑 γpop]"...
+        iMod (mono_deque_update_bot _ (b2-1) with "MD") as "MD"...
+      iMod ("Commit" $! (slice l t2 (b2-1)) true v with "[Cont]") as "Φ"...
+      iModIntro. iModIntro. iSplitL "t↦ b↦ arr↦ γq γpop MD". 1: fr...
+      wp_pures. case_bool_decide... wp_pures.
+      (* read [b2-1] *)
+      wp_bind (! _)%E.
+      iApply (wp_load_offset with "arr👑")... iNext. iIntros "arr👑".
+      wp_pures. case_bool_decide... wp_pures. iApply "Φ". fr. }
+
+    (* otherwise... *)
+    wp_load. iModIntro. iSplitL "t↦ b↦ arr↦ γpop γq MD". 1: fr.
+    wp_pures.
+
+    (* empty *)
+    case_bool_decide as Hbt; wp_pures.
+    { wp_bind (_ <- _)%E.
+      iInv "Inv" as (t3 b3 l3 Pop4)
+        ">(%BOUND3 & t↦ & b↦ & arr↦ & γq & γpop & MD)".
+        iDestruct (ghost_var_agree with "γ👑 γpop") as "%". subst.
+        iDestruct (mapsto_agree with "b↦ b👑") as "%".
+          injection H as [=]. assert (b2 = b3); subst... clear H.
+        iDestruct (array_agree with "arr↦ arr👑") as "%"; subst...
+      replace t2 with b3...
+      (* roll back bot *)
+      iCombine "b👑 b↦" as "b↦". wp_store.
+        iDestruct "b↦" as "[b👑 b↦]".
+        iMod (ghost_var_update_2 false with "γ👑 γpop") as "[γ👑 γpop]"...
+      (* AU *)
+      iMod "AU" as (l') "[Cont [_ Commit]]".
+      iMod ("Commit" $! l' false #() with "[Cont]") as "Φ"...
+      iSplitL "t↦ b↦ arr↦ γpop γq MD". 1: fr.
+      iModIntro. wp_pures. iApply "Φ". fr. }
+    
+    (* read [b2-1] *)
+    wp_bind (! _)%E.
+    assert (is_Some (l !! (b2-1))) as [v Hv]...
+    iApply (wp_load_offset with "arr👑")... iNext. iIntros "arr👑".
+    wp_pures.
+
+    (* cas top, we already handled normal pop *)
+    case_bool_decide... clear H. wp_pures.
+    wp_bind (CmpXchg _ _ _)%E.
+    iInv "Inv" as (t3 b3 l3 Pop3)
+      ">(%BOUND3 & t↦ & b↦ & arr↦ & γq & γpop & MD)".
+      iDestruct (ghost_var_agree with "γ👑 γpop") as "%". subst.
+      iDestruct (mapsto_agree with "b↦ b👑") as "%".
+        injection H as [=]. assert (b2 = b3); subst... clear H.
+      iDestruct (array_agree with "arr↦ arr👑") as "%"... subst.
+    assert (t2 = b3-1)... subst. clear n Hbt.
+    replace (Z.of_nat (b3-1) + 1)%Z with (Z.of_nat b3)...
+    destruct (decide (b3-1 = t3)).
+    - (* success *)
+      subst. wp_cmpxchg_suc.
+
+      (* AU *)
+      iMod "AU" as (l') "[Cont [_ Commit]]".
+        unfold deque_content.
+        iDestruct (ghost_var_agree with "Cont γq") as "%". subst.
+      erewrite slice_shrink_left... rewrite slice_to_nil...
+      iMod (ghost_var_update_2 [] with "Cont γq") as "[Cont γq]"...
+      iMod (mono_deque_update_top _ b3 with "MD") as "MD"...
+      iMod ("Commit" $! [] true v with "[Cont]") as "Φ"...
+      iModIntro. iSplitL "t↦ b↦ arr↦ γpop γq MD".
+        { fr. rewrite slice_to_nil... fr... }
+      wp_pures.
+
+      (* store bot *)
+      replace (Z.of_nat (b3-1) + 1)%Z with (Z.of_nat b3)...
+      wp_bind (_ <- _)%E.
+      iInv "Inv" as (t4 b4 l4 Pop4)
+        ">(%BOUND4 & t↦ & b↦ & arr↦ & γq & γpop & MD)".
+        iDestruct (ghost_var_agree with "γ👑 γpop") as "%". subst.
+        iDestruct (mapsto_agree with "b↦ b👑") as "%".
+          injection H as [=]. assert (b3 = b4) by lia. subst. clear H.
+        iDestruct (array_agree with "arr↦ arr👑") as "%"... subst.
+      iCombine "b👑 b↦" as "b↦". wp_store.
+        iDestruct "b↦" as "[b👑 b↦]".
+      iMod (ghost_var_update_2 false with "γ👑 γpop") as "[γ👑 γpop]"...
+      iModIntro. iSplitL "t↦ b↦ arr↦ γpop γq MD". 1: fr.
+      wp_pures. iApply "Φ". fr.
+    - (* fail *)
+      wp_cmpxchg_fail. { intro. injection H... }
+      iMod "AU" as (l') "[Cont [_ Commit]]".
+      iMod ("Commit" $! l' false #() with "[Cont]") as "Φ"...
+      iModIntro. iSplitL "t↦ b↦ arr↦ γpop γq MD". 1: fr.
+      wp_pures.
+
+      (* store bot *)
+      replace (Z.of_nat (b3-1) + 1)%Z with (Z.of_nat b3)...
+      wp_bind (_ <- _)%E.
+      iInv "Inv" as (t4 b4 l4 Pop4)
+        ">(%BOUND4 & t↦ & b↦ & arr↦ & γq & γpop & MD)".
+        iDestruct (ghost_var_agree with "γ👑 γpop") as "%". subst.
+        iDestruct (mapsto_agree with "b↦ b👑") as "%".
+          injection H as [=]. assert (b3 = b4) by lia. subst. clear H.
+        iDestruct (array_agree with "arr↦ arr👑") as "%"... subst.
+      iCombine "b👑 b↦" as "b↦". wp_store.
+        iDestruct "b↦" as "[b👑 b↦]".
+      iMod (ghost_var_update_2 false with "γ👑 γpop") as "[γ👑 γpop]"...
+      iModIntro. iSplitL "t↦ b↦ arr↦ γpop γq MD". 1: fr.
+      wp_pures. iApply "Φ". fr.
+  Qed.
+
+  Lemma steal_spec γq γpop γm q :
+    is_deque γq γpop γm q -∗
+    <<< ∀∀ l : list val, deque_content γq l >>>
+      steal q @ ↑N
+    <<< ∃∃ (l' : list val) (b : bool) (v : val),
+        deque_content γq l' ∗
+        ⌜l = if b then [v]++l' else l'⌝ ,
+      RET (#b, v) >>>.
+  Proof with autoall.
+    iIntros "#Is" (Φ) "AU".
+      iDestruct "Is" as (arr top bot) "[%Is Inv]". subst.
+    wp_lam. unfold code.arr, code.top, code.bot. wp_pures.
+
+    (* load top *)
+    wp_bind (! _)%E.
+    iInv "Inv" as (t1 b1 l1 Pop1)
+      ">(%BOUND1 & t↦ & b↦ & arr↦ & γq & γpop & MD)".
+      iDestruct (mono_deque_get_lb with "MD") as "#MDlb1".
+    wp_load.
+    iModIntro. iSplitL "t↦ b↦ arr↦ γq γpop MD". 1: fr.
+    wp_pures.
+
+    (* load bot *)
+    wp_bind (! _)%E.
+    iInv "Inv" as (t2 b2 l2 Pop2)
+      ">(%BOUND2 & t↦ & b↦ & arr↦ & γq & γpop & MD)".
+      iDestruct (mono_deque_get_lb with "MD") as "#MDlb2".
+      iDestruct (mono_deque_auth_lb_top with "MD MDlb1") as "%Ht12".
+    wp_load.
+    iModIntro. iSplitL "t↦ b↦ arr↦ γq γpop MD". 1: fr.
+    wp_pures.
+
+    (* no chance to steal *)
+    case_bool_decide; wp_pures.
+    { iMod "AU" as (l) "[Cont [_ Commit]]".
+      iMod ("Commit" $! l false #() with "[Cont]") as "Φ"...
+      iApply "Φ"... }
+    assert (t1 < b2) as Htb12. 1: destruct Pop2... clear H.
+
+    (* read [t1] *)
+    wp_bind (! _)%E.
+    iInv "Inv" as (t3 b3 l3 Pop3)
+      ">(%BOUND3 & t↦ & b↦ & arr↦ & γq & γpop & MD)".
+      iDestruct (mono_deque_get_lb with "MD") as "#MDlb3".
+      iDestruct (mono_deque_auth_lb_top with "MD MDlb2") as "%Ht23".
+    assert (is_Some (l3 !! t1)) as [v Hv]...
+    iApply (wp_load_offset with "arr↦")... iNext. iIntros "arr↦".
+    iModIntro. iSplitL "t↦ b↦ arr↦ γq γpop MD". 1: fr.
+    wp_pures.
+
+    (* cas top *)
+    wp_bind (CmpXchg _ _ _)%E.
+    iInv "Inv" as (t4 b4 l4 Pop4)
+      ">(%BOUND4 & t↦ & b↦ & arr↦ & γq & γpop & MD)".
+      iDestruct (mono_deque_auth_lb_top with "MD MDlb3") as "%Ht34".
+    destruct (decide (t1 = t4)).
+    - (* success *)
+      assert (t1 = t2)... assert (t2 = t3)... subst.
+      assert (t3 < b3) as Htb3... assert (t3 < b4) as Htb4...
+      wp_cmpxchg_suc.
+      replace (Z.of_nat t3 + 1)%Z with (Z.of_nat (S t3))...
+      (* update ghost *)
+      iDestruct (mono_deque_get_lb with "MD") as "#MDlb4".
+      iDestruct (mono_deque_lb_lookup _ t3 with "MDlb3 MDlb4") as "%"...
+        rewrite Hv in H.
+      iMod (mono_deque_update_top _ (S t3) with "MD") as "MD"...
+      (* AU *)
+      iMod "AU" as (l') "[Cont [_ Commit]]".
+        unfold deque_content.
+        iDestruct (ghost_var_agree with "γq Cont") as "%". subst.
+      iMod (ghost_var_update_2 (slice l4 (S t3) b4) with "γq Cont") as "[γq Cont]"...
+      iMod ("Commit" $! (slice l4 (S t3) b4) true v with "[Cont]") as "Φ".
+        { fr. erewrite slice_shrink_left... }
+      iModIntro. iSplitL "t↦ b↦ arr↦ γq γpop MD". 1: fr...
+      wp_pures. iApply "Φ"...
+    - (* fail *)
+      wp_cmpxchg_fail. { intro. injection H... }
+      iMod "AU" as (l) "[Cont [_ Commit]]".
+      iMod ("Commit" $! l false #() with "[Cont]") as "Φ"...
+      iModIntro. iSplitL "t↦ b↦ arr↦ γq γpop MD". 1: fr.
+      wp_pures. iApply "Φ"...
+  Qed.
+End proof.
